src/program_proof/memkv/memkv_coord_clerk_proof.v
@@ -5,7 +5,7 @@ From Perennial.program_proof.memkv Require Import common_proof memkv_shard_clerk
 
 Section memkv_coord_clerk_proof.
 
-Context `{!heapG Σ, rpcG Σ memkv_marshal_get_proof.GetReplyC, rpcregG Σ, kvMapG Σ}.
+Context `{!heapG Σ, rpcG Σ ShardReplyC, rpcregG Σ, kvMapG Σ}.
 
 Axiom own_MemKVCoordClerk : loc → iProp Σ.
 
