src/program_proof/memkv/memkv_marshal_conditional_put_proof.v
@@ -1,0 +1,111 @@
+From Perennial.program_proof Require Import dist_prelude.
+From Goose.github_com.mit_pdos.gokv Require Import memkv.
+From Perennial.program_proof Require Import marshal_proof.
+
+(*
+  Defines Coq request and reply types for shard server Put RPC. Also defines
+  has_encoding for Put Request/Reply and provides WPs for {de|en}codePutRe{ply|quest}()
+ *)
+
+Section memkv_marshal_conditional_put_proof.
+
+Context `{!heapG Σ}.
+
+Record ConditionalPutRequestC := mkConditionalPutRequestC {
+  CPR_CID : u64;
+  CPR_Seq : u64;
+  CPR_Key : u64;
+  CPR_ExpValue : list u8;
+  CPR_NewValue : list u8;
+}.
+
+Record ConditionalPutReplyC := mkConditionalPutReplyC {
+  CPR_Err : u64;
+  CPR_Succ : bool;
+}.
+
+Definition own_ConditionalPutRequest args_ptr expv_sl newv_sl args : iProp Σ :=
+  "HCID" ∷ args_ptr ↦[ConditionalPutRequest :: "CID"] #args.(CPR_CID) ∗
+  "HSeq" ∷ args_ptr ↦[ConditionalPutRequest :: "Seq"] #args.(CPR_Seq) ∗
+  "HKey" ∷ args_ptr ↦[ConditionalPutRequest :: "Key"] #args.(CPR_Key) ∗
+  "HExpValue" ∷ args_ptr ↦[ConditionalPutRequest :: "ExpectedValue"] (slice_val expv_sl) ∗
+  "HNewValue" ∷ args_ptr ↦[ConditionalPutRequest :: "NewValue"] (slice_val newv_sl) ∗
+  "HExpValue_sl" ∷ typed_slice.is_slice expv_sl byteT 1%Qp args.(CPR_ExpValue) ∗
+  "HNewValue_sl" ∷ typed_slice.is_slice newv_sl byteT 1%Qp args.(CPR_NewValue) ∗
+  "%HseqPositive" ∷ ⌜int.Z args.(CPR_Seq) > 0⌝
+.
+
+Definition own_ConditionalPutReply reply_ptr rep : iProp Σ :=
+  "HErr" ∷ reply_ptr ↦[ConditionalPutReply :: "Err"] #rep.(CPR_Err) ∗
+  "HSucc" ∷ reply_ptr ↦[ConditionalPutReply :: "Success"] #rep.(CPR_Succ)
+.
+
+Definition has_encoding_ConditionalPutRequest (data:list u8) (args:ConditionalPutRequestC) : Prop :=
+  has_encoding data [ EncUInt64 args.(CPR_CID) ; EncUInt64 args.(CPR_Seq); EncUInt64 args.(CPR_Key);
+    EncUInt64 (length args.(CPR_ExpValue)) ; EncBytes args.(CPR_ExpValue);
+    EncUInt64 (length args.(CPR_NewValue)) ; EncBytes args.(CPR_NewValue)  ].
+
+Definition has_encoding_ConditionalPutReply (data:list u8) (rep:ConditionalPutReplyC) :=
+  has_encoding data [ EncUInt64 rep.(CPR_Err); EncBool rep.(CPR_Succ) ].
+
+Lemma wp_encodeConditionalPutRequest args_ptr expv_sl newv_sl args :
+  {{{
+       own_ConditionalPutRequest args_ptr expv_sl newv_sl args
+  }}}
+    encodeConditionalPutRequest #args_ptr
+  {{{
+       (reqData:list u8) req_sl, RET (slice_val req_sl); ⌜has_encoding_ConditionalPutRequest reqData args⌝ ∗
+         typed_slice.is_slice req_sl byteT 1%Qp reqData ∗
+         own_ConditionalPutRequest args_ptr expv_sl newv_sl args
+  }}}.
+Proof.
+Admitted.
+
+Lemma wp_decodeConditionalPutRequest req_sl reqData args :
+  {{{
+       ⌜has_encoding_ConditionalPutRequest reqData args⌝ ∗
+       typed_slice.is_slice req_sl byteT 1%Qp reqData
+  }}}
+    decodeConditionalPutRequest (slice_val req_sl)
+  {{{
+       (args_ptr:loc) expv_sl newv_sl, RET #args_ptr; own_ConditionalPutRequest args_ptr expv_sl newv_sl args
+  }}}.
+Proof.
+Admitted.
+
+Lemma has_encoding_ConditionalPutRequest_inj (reqRaw:list u8) req req' :
+  has_encoding_ConditionalPutRequest reqRaw req →
+  has_encoding_ConditionalPutRequest reqRaw req' →
+  req = req'.
+Proof.
+  intros.
+  unfold has_encoding_ConditionalPutRequest in *.
+Admitted.
+
+Lemma wp_decodeConditionalPutReply rep rep_sl repData :
+  {{{
+       typed_slice.is_slice rep_sl byteT 1%Qp repData ∗
+       ⌜has_encoding_ConditionalPutReply repData rep ⌝
+  }}}
+    decodeConditionalPutReply (slice_val rep_sl)
+  {{{
+       (rep_ptr:loc) , RET #rep_ptr;
+       own_ConditionalPutReply rep_ptr rep
+  }}}.
+Proof.
+Admitted.
+
+Lemma wp_encodeConditionalPutReply rep_ptr rep :
+  {{{
+       own_ConditionalPutReply rep_ptr rep
+  }}}
+    encodeConditionalPutReply #rep_ptr
+  {{{
+       repData rep_sl, RET (slice_val rep_sl);
+       typed_slice.is_slice rep_sl byteT 1%Qp repData ∗
+       ⌜has_encoding_ConditionalPutReply repData rep ⌝
+  }}}.
+Proof.
+Admitted.
+
+End memkv_marshal_conditional_put_proof.
