src/program_proof/memkv/memkv_move_shard_proof.v
@@ -5,7 +5,7 @@ From Perennial.program_proof.memkv Require Export memkv_shard_definitions memkv_
 
 Section memkv_move_shard_proof.
 
-Context `{!heapG Σ, rpcG Σ GetReplyC, rpcregG Σ, kvMapG Σ}.
+Context `{!heapG Σ, rpcG Σ ShardReplyC, rpcregG Σ, kvMapG Σ}.
 
 Lemma wp_MoveShardRPC (s args_ptr:loc) args γsh γ :
   is_MemKVShardServer s γ -∗
